YoungDiagram/Mutations/MixA.lean
@@ -1,1 +1,296 @@
 import YoungDiagram
+
+open Chromosome
+
+variable {ε : GeneType} {m n : ℕ}
+
+local notation "type4X" => Gene.ofRank m GeneType.NonPolarized + Gene.ofRank n GeneType.NonPolarized
+local notation "type4Y" => Gene.ofRank (m - 1) ε + Gene.ofRank (n + 1) (- ε)
+
+local notation "type5X" => Gene.ofRank m GeneType.NonPolarized + Gene.ofRank n ε
+local notation "type5Y" => Gene.ofRank (m - 1) ε + Gene.ofRank (n + 1) GeneType.NonPolarized
+
+local notation "type6X" => Gene.ofRank m ε + Gene.ofRank n GeneType.NonPolarized
+local notation "type6Y" => Gene.ofRank (m - 1) GeneType.NonPolarized + Gene.ofRank (n + 1) ε
+
+local notation "type7X" => Gene.ofRank m ε + Gene.ofRank n (- ε)
+local notation "type7Y" => Gene.ofRank (m - 1) GeneType.NonPolarized +
+  Gene.ofRank (n + 1) GeneType.NonPolarized
+
+local notation "type8X" => Gene.ofRank m ε + Gene.ofRank n ε
+local notation "type8Y" => Gene.ofRank (m - 2) ε + Gene.ofRank (n + 2) ε
+
+#exit
+
+section Aux
+
+section type4_isMutation
+
+lemma mutation_type4_ne (h_le : m ≤ n) (hm : 1 ≤ m) : type4X ≠ type4Y := by
+  sorry
+
+lemma mutation_type4_iterate_signature_eq (hε : ε ≠ .NonPolarized)
+  (h_le : m ≤ n) (hm : 1 ≤ m) (i k : ℕ) (hi : i ≤ k) :
+    (prime^[i] (Gene.ofRank (m + k) .NonPolarized + Gene.ofRank (n + k) .NonPolarized)).signature =
+    (prime^[i] (Gene.ofRank (m + k - 1) ε + Gene.ofRank (n + k + 1) (- ε))).signature := by
+  sorry
+
+lemma mutation_type4_signature_eq (hε : ε ≠ .NonPolarized) (h_le : m ≤ n) (hm : 1 ≤ m) :
+    signature type4X = signature type4Y := by
+  sorry
+
+lemma mutation_type4_le (hε : ε ≠ .NonPolarized) (h_le : m ≤ n) : type4X ≤ type4Y := by
+  sorry
+
+end type4_isMutation
+
+section type5_isMutation
+
+lemma mutation_type5_ne (h_le : m < n) (hm : 1 ≤ m) : type5X ≠ type5Y := by
+  sorry
+
+lemma mutation_type5_iterate_signature_eq (hε : ε ≠ .NonPolarized)
+  (h_le : m < n) (hm : 1 ≤ m) (i k : ℕ) (hi : i ≤ k) :
+    (prime^[i] (Gene.ofRank (m + k) .NonPolarized + Gene.ofRank (n + k) ε)).signature =
+    (prime^[i] (Gene.ofRank (m + k - 1) ε + Gene.ofRank (n + k + 1) .NonPolarized)).signature := by
+  sorry
+
+lemma mutation_type5_signature_eq (hε : ε ≠ .NonPolarized) (h_le : m < n) (hm : 1 ≤ m) :
+    signature type5X = signature type5Y := by
+  sorry
+
+lemma mutation_type5_le (hε : ε ≠ .NonPolarized) (h_le : m < n) : type5X ≤ type5Y := by
+  sorry
+
+end type5_isMutation
+
+section type6_isMutation
+
+lemma mutation_type6_ne (h_le : m < n) (hm : 1 ≤ m) : type6X ≠ type6Y := by
+  sorry
+
+lemma mutation_type6_iterate_signature_eq (hε : ε ≠ .NonPolarized)
+  (h_le : m < n) (hm : 1 ≤ m) (i k : ℕ) (hi : i ≤ k) :
+    (prime^[i] (Gene.ofRank (m + k) ε + Gene.ofRank (n + k) .NonPolarized)).signature =
+    (prime^[i] (Gene.ofRank (m + k - 1) .NonPolarized + Gene.ofRank (n + k + 1) ε)).signature := by
+  sorry
+
+lemma mutation_type6_signature_eq (hε : ε ≠ .NonPolarized) (h_le : m < n) (hm : 1 ≤ m) :
+    signature type6X = signature type6Y := by
+  sorry
+
+lemma mutation_type6_le (hε : ε ≠ .NonPolarized) (h_le : m < n) : type6X ≤ type6Y := by
+  sorry
+
+end type6_isMutation
+
+section type7_isMutation
+
+lemma mutation_type7_ne (h_le : m ≤ n) (hm : 1 ≤ m) : type7X ≠ type7Y := by
+  sorry
+
+lemma mutation_type7_iterate_signature_eq (hε : ε ≠ .NonPolarized)
+  (h_le : m ≤ n) (hm : 1 ≤ m) (i k : ℕ) (hi : i ≤ k) :
+    (prime^[i] (Gene.ofRank (m + k) ε + Gene.ofRank (n + k) (- ε))).signature =
+    (prime^[i] (Gene.ofRank (m + k - 1) .NonPolarized +
+      Gene.ofRank (n + k + 1) .NonPolarized)).signature := by
+  sorry
+
+lemma mutation_type7_signature_eq (hε : ε ≠ .NonPolarized) (h_le : m ≤ n) (hm : 1 ≤ m) :
+    signature type7X = signature type7Y := by
+  sorry
+
+lemma mutation_type7_le (hε : ε ≠ .NonPolarized) (h_le : m ≤ n) : type7X ≤ type7Y := by
+  sorry
+
+end type7_isMutation
+
+section type8_isMutation
+
+lemma mutation_type8_ne (h_le : m ≤ n) (hm : 1 < m) : type8X ≠ type8Y := by
+  sorry
+
+lemma mutation_type8_iterate_signature_eq (hε : ε ≠ .NonPolarized)
+  (h_le : m ≤ n) (hm : 1 < m) (i k : ℕ) (hi : i ≤ k) :
+    (prime^[i] (Gene.ofRank (m + k) ε + Gene.ofRank (n + k) ε)).signature =
+    (prime^[i] (Gene.ofRank (m + k - 2) ε + Gene.ofRank (n + k + 2) ε)).signature := by
+  sorry
+
+lemma mutation_type8_signature_eq (hε : ε ≠ .NonPolarized) (h_le : m ≤ n) (hm : 1 < m) :
+    signature type8X = signature type8Y := by
+  sorry
+
+lemma mutation_type8_le (hε : ε ≠ .NonPolarized) (h_le : m ≤ n) (hm : 1 < m) :
+    type8X ≤ type8Y := by
+  sorry
+
+end type8_isMutation
+
+end Aux
+
+open Variety
+
+namespace MixA
+
+variable (hε : ε ≠ .NonPolarized)
+
+noncomputable section type4
+
+variable (hle : m ≤ n) (hm : 1 ≤ m)
+
+def X4 : Mix (Pi, Lambda) := by
+  use type4X
+  have hle := hle
+  have hm := hm
+  have hε := hε
+  sorry
+
+def X4' : Mix (Lambda, Pi) := by
+  use type4X
+  have hle := hle
+  have hm := hm
+  have hε := hε
+  sorry
+
+lemma X4_eq : X4 hε hle hm =
+  Gene.ofRank m .NonPolarized + Gene.ofRank n .NonPolarized := rfl
+
+lemma X4'_eq : X4' hε hle hm =
+  Gene.ofRank m .NonPolarized + Gene.ofRank n .NonPolarized := rfl
+
+def Y4 : Mix (Pi, Lambda) := by
+  use type4Y
+  have hle := hle
+  have hm := hm
+  have hε := hε
+  sorry
+
+def Y4 : Mix (Pi, Lambda) := by
+  use type4Y
+  have hle := hle
+  have hm := hm
+  have hε := hε
+  sorry
+
+#exit
+
+lemma X1_eq : X1 hε hle hm =
+  Gene.ofRank m ε + Gene.ofRank n (- ε) := rfl
+
+def Y1 : Pi := by
+  use type1Y
+  rw [mem_Pi_iff, IsPolarized_iff_add]
+  refine ⟨?_, by rwa [IsPolarized_ofRank (Nat.le_add_left 1 n)]⟩
+  match m with
+  | 1 =>
+    rw [← mem_Pi_iff, Nat.sub_self, Gene.ofRank_zero]
+    exact zero_mem _
+  | m + 2 =>
+    rwa [IsPolarized_ofRank (Nat.le_of_ble_eq_true rfl),
+      ← GeneType.neg_ne_nonPolarized_iff]
+
+lemma Y1_eq : Y1 hε hle hm =
+  Gene.ofRank (m - 1) (- ε) + Gene.ofRank (n + 1) ε := rfl
+
+end type1
+
+noncomputable section type2
+
+variable (hle : m ≤ n) (hm : 1 < m)
+
+def X2 : Pi := by
+  use type2X
+  rw [mem_Pi_iff, IsPolarized_iff_add]
+  exact ⟨by rwa [IsPolarized_ofRank (le_of_lt hm)],
+    by rwa [IsPolarized_ofRank ((le_of_lt hm).trans hle)]⟩
+
+lemma X2_eq : X2 hε hle hm =
+  Gene.ofRank m ε + Gene.ofRank n ε := rfl
+
+def Y2 : Pi := by
+  use type2Y
+  rw [mem_Pi_iff, IsPolarized_iff_add]
+  refine ⟨?_, by rwa [IsPolarized_ofRank (Nat.le_add_left 1 (n + 1))]⟩
+  match m with
+  | 2 =>
+    rw [← mem_Pi_iff, Nat.sub_self, Gene.ofRank_zero]
+    exact zero_mem _
+  | m + 3 => rwa [IsPolarized_ofRank (by omega)]
+
+lemma Y2_eq : Y2 hε hle hm =
+  Gene.ofRank (m - 2) ε + Gene.ofRank (n + 2) ε := rfl
+
+end type2
+
+noncomputable section type3
+
+variable (hle : m ≤ n) (hm : 1 ≤ m)
+
+def X3 : Pi := by
+  use type3X
+  rw [mem_Pi_iff, IsPolarized_iff_add]
+  exact ⟨by rwa [IsPolarized_ofRankAlt hm], by
+    rwa [IsPolarized_ofRankAlt (hm.trans hle),
+      ← GeneType.neg_ne_nonPolarized_iff]⟩
+
+lemma X3_eq : X3 hε hle hm =
+  Gene.ofRankAlt m ε + Gene.ofRankAlt n (- ε) := rfl
+
+def Y3 : Pi := by
+  use type3Y
+  rw [mem_Pi_iff, IsPolarized_iff_add]
+  refine ⟨?_, by rwa [IsPolarized_ofRankAlt (by omega)]⟩
+  match m with
+  | 1 =>
+    rw [Nat.sub_self, Gene.ofRankAlt_def, Gene.ofRank_zero, ← mem_Pi_iff]
+    exact zero_mem _
+  | m + 2 => rwa [IsPolarized_ofRankAlt (by omega),
+    GeneType.neg_ne_nonPolarized_iff, neg_neg]
+
+lemma Y3_eq : Y3 hε hle hm =
+  Gene.ofRankAlt (m - 1) (- ε) + Gene.ofRankAlt (n + 1) ε := rfl
+
+end type3
+
+inductive Primitive : Pi → Pi → Prop
+  | type1 (ε : GeneType) (hε : ε ≠ .NonPolarized)
+    {m n : ℕ} (hle : m ≤ n) (hm : 1 ≤ m) :
+      Primitive (X1 hε hle hm) (Y1 hε hle hm)
+  | type2 (ε : GeneType) (hε : ε ≠ .NonPolarized)
+    {m n : ℕ} (hle : m ≤ n) (hm : 1 < m) :
+      Primitive (X2 hε hle hm) (Y2 hε hle hm)
+  | type3 (ε : GeneType) (hε : ε ≠ .NonPolarized)
+    {m n : ℕ} (hle : m ≤ n) (hm : 1 ≤ m) :
+      Primitive (X3 hε hle hm) (Y3 hε hle hm)
+
+inductive Step : Pi → Pi → Prop
+  | mk (X Y Z : Pi) (h : Primitive X Y) :
+      Step (X + Z) (Y + Z)
+
+lemma Primitive.isMutation {X Y : Pi} (h : Pi.Primitive X Y) :
+    IsMutation X Y := by
+  cases h with
+  | type1 ε hε hle hm =>
+    exact ⟨mutation_type1_le hε hle,
+      mutation_type1_ne hle hm, mutation_type1_signature_eq hε hle hm⟩
+  | type2 ε hε hle hm =>
+    exact ⟨mutation_type2_le hε hle hm,
+      mutation_type2_ne hle hm, mutation_type2_signature_eq hε hle hm⟩
+  | type3 ε hε hle hm =>
+    exact ⟨mutation_type3_le hε hle hm,
+      mutation_type3_ne hle hm, mutation_type3_signature_eq hε hle hm⟩
+
+lemma Step.isMutation {X Y : Pi} (h : Pi.Step X Y) :
+    IsMutation X Y := by
+  cases h with
+  | mk X Y Z h =>
+    exact .add_right _ (Pi.Primitive.isMutation h)
+
+lemma Step.add_right_pi (W : Variety.Pi) {A B : Variety.Pi}
+    (h : Pi.Step A B) : Pi.Step (A + W) (B + W) := by
+  cases h with
+  | mk X Y Z hPrim =>
+    rw [add_assoc, add_assoc]
+    exact Pi.Step.mk X Y (Z + W) hPrim
+
+end Pi
